\begin{excercise}\label{e1}
    Prove the following results.
    For proximal point method, if $f$ is closed and convex and optimal value $f^*$ is finite and attained at $\xB_*$. We have
    \[
    f(\xB_k) - f^* \leq \frac{ \norm{\xB_0 - \xB_*}^2_2 }{ 2 \sum_{i=0}^{k-1} t_i}, \quad\textrm{for } k \geq 1.
    \]
\end{excercise}
    
\begin{PROOF}{e1}
    \begin{lemma}\label{lemma:e1-1}
        \(\uB = \prox_h(\xB)\) is equivalent to the following 
        \begin{enumerate}
            \item \(\xB - \uB \in \partial h(\uB)\),
            \item \(h(\zB) \ge h(\uB) + (\xB - \uB)^\top (\zB - \uB)\) for all \(\zB\).
        \end{enumerate}
    \end{lemma}

    The updating rule of proximal point method can be concluded as 
    \[
        \xB' = \prox_{tf}(\xB).
    \]
    According to Lemma.~\ref{lemma:e1-1}, we can obtain
    \[
        f(\zB) \ge f(\xB') + \frac{1}{t}(\xB - \xB')^\top (\zB - \xB')
    \]
    Let \(\zB = \xB\), we can obtain
    \[
        f(\xB') \le f(\xB) - \frac{1}{t}\norm{\xB - \xB'}^2_2.  
    \]
    Therefore, this algorithm is a descent method. Let \(\zB = \xB_*\), we can get
    \[
        \begin{aligned}
            f(\xB') - f(\xB_*) &\le \frac{1}{t} (\xB - \xB')^\top(\xB' - \xB_*) \\
            &= \frac{1}{t} [(\xB - \xB_*) - (\xB' - \xB_*)]^\top (\xB' - \xB_*) \\
            &= \frac{1}{t} \left[ (\xB - \xB_*)^\top(\xB' - \xB_*) - \norm{\xB' - \xB_*}_2^2 \right]\\
            &\le \frac{1}{t} \left[\norm{\xB - \xB_*}_2\norm{\xB' - \xB_*}_2 - \norm{\xB' - \xB_*}_2^2 \right]\\
            &\le \frac{1}{t} \left[\frac{\norm{\xB - \xB_*}_2^2 + \norm{\xB' - \xB_*}_2^2}{2} - \norm{\xB' - \xB_*}_2^2 \right]\\
            &= \frac{1}{2t}\left(\norm{\xB - \xB_*}_2^2 - \norm{\xB' - \xB_*}_2^2  \right)
        \end{aligned}
    \]
    Let \(t = t_i\), \(\xB = \xB_i\), \(\xB' = \xB_{i+1}\). For \(i = 0, \dots, k-1\)
    \[
        t_i (f(\xB_{i+1}) - f(\xB_*)) \le \frac{1}{2} \left( 
            \norm{\xB_i - \xB_*}_2^2 + \norm{\xB_{i+1} - \xB_*}_2^2
        \right).
    \]
    Adding inequalities from \(i = 0\) to \(k-1\) gives
    \[
        \left( \sum_{i=0}^{k-1} t_i \right) (f(\xB_k) - f(\xB_*)) \le
        \sum_{i=0}^{k-1} t_i (f(\xB_{i+1}) - f(\xB_*)) \le \frac{1}{2} \norm{\xB_0 - \xB_*}_2^2.
    \]
    Thus we have \(f(\xB_k) - f^* \leq ( \norm{\xB_0 - \xB_*}^2_2 ) /{ (2 \sum_{i=0}^{k-1} t_i})\) for \(k \ge 1\).
\end{PROOF}